src/program_proof/session/processRequest.v
@@ -3,16 +3,13 @@ From Perennial.program_proof.session Require Export versionVector processClientR
 
 Section heap.
 
-  Definition SERVER_INVARIANT (s: Server.t) : Prop :=
-    is_sorted s.(Server.PendingOperations) /\ is_sorted s.(Server.OperationsPerformed) /\ length s.(Server.VectorClock) < uint.nat s.(Server.Id).
-
   Context `{hG: !heapGS Σ}.
 
   Lemma wp_processClientRequest sv s msgv msg (n: nat) (m: nat) len_po len_ga len_c2s len_s2c :
     {{{
         is_server sv s n m m m len_po len_ga ∗
         is_message msgv msg n len_c2s len_s2c ∗
-        ⌜m = len_c2s /\ SERVER_INVARIANT s⌝
+        ⌜m = len_c2s /\ INVARIANT.SERVER s⌝
     }}}
       processClientRequest (server_val sv) (message_val msgv)
     {{{
@@ -21,10 +18,10 @@ Section heap.
         is_server ns (coq_processClientRequest s msg).1.2 n m m m len_po len_ga ∗
         is_message nm (coq_processClientRequest s msg).2 n 0%nat (if b then len_c2s else 0%nat) ∗
         is_message msgv msg n len_c2s len_s2c ∗
-        ⌜SERVER_INVARIANT (coq_processClientRequest s msg).1.2⌝
+        ⌜INVARIANT.SERVER (coq_processClientRequest s msg).1.2⌝
     }}}.
-  Proof. (**
-    rewrite redefine_server_val redefine_message_val. TypeVector.des sv. TypeVector.des msgv. iIntros "%Φ (H_server & H_message & %H1_precondition & %H2_precondition) HΦ".
+  Proof.
+    rewrite redefine_server_val redefine_message_val. TypeVector.des sv. TypeVector.des msgv. iIntros "%Φ (H_server & H_message & %H1_precondition & %H2_precondition) HΦ". destruct H2_precondition as [? ? ? ?].
     iDestruct "H_server" as "(%H1 & %H2 & H3 & H4 & %H5 & H6 & H7 & H8 & H9 & %H10)".
     iDestruct "H_message" as "(%H11 & %H12 & %H13 & %H14 & %H15 & H16 & %H17 & %H18 & %H19 & H20 & %H21 & %H22 & %H23 & %H24 & %H25 & %H26 & H27 & %H28 & %H29 & %H30)".
     simplNotation. subst. rewrite /processClientRequest.
@@ -37,7 +34,6 @@ Section heap.
       set (nm := (W64 0, W64 0, W64 0, W64 0, W64 0, Slice.nil, W64 0, W64 0, Slice.nil, W64 0, W64 0, W64 0, W64 0, W64 0, W64 0, Slice.nil, W64 0, W64 0)).
       replace (Φ (#false, (#s .(Server.Id), (#s .(Server.NumberOfServers), (t4, (t3, (t2, (t1, (t0, (t, #())))))))), (zero_val uint64T, (zero_val uint64T, (zero_val uint64T, (zero_val uint64T, (zero_val uint64T, (zero_val (slice.T uint64T), (zero_val uint64T, (zero_val uint64T, (zero_val (slice.T (slice.T uint64T * (uint64T * unitT)%ht)), (zero_val uint64T, (zero_val uint64T, (zero_val uint64T, (zero_val uint64T, (zero_val uint64T, (zero_val uint64T, (zero_val (slice.T uint64T), (zero_val uint64T, (zero_val uint64T, #())))))))))))))))))))%V) with (Φ (#b, (#ns.1.1.1.1.1.1.1, (#ns.1.1.1.1.1.1.2, (ns.1.1.1.1.1.2, (ns.1.1.1.1.2, (ns.1.1.1.2, (ns.1.1.2, (ns.1.2, (ns.2, #())))))))), (#nm.1.1.1.1.1.1.1.1.1.1.1.1.1.1.1.1.1, (#nm.1.1.1.1.1.1.1.1.1.1.1.1.1.1.1.1.2, (#nm.1.1.1.1.1.1.1.1.1.1.1.1.1.1.1.2, (#nm.1.1.1.1.1.1.1.1.1.1.1.1.1.1.2, (#nm.1.1.1.1.1.1.1.1.1.1.1.1.1.2, (nm.1.1.1.1.1.1.1.1.1.1.1.1.2, (#nm.1.1.1.1.1.1.1.1.1.1.1.2, (#nm.1.1.1.1.1.1.1.1.1.1.2, (nm.1.1.1.1.1.1.1.1.1.2, (#nm.1.1.1.1.1.1.1.1.2, (#nm.1.1.1.1.1.1.1.2, (#nm.1.1.1.1.1.1.2, (#nm.1.1.1.1.1.2, (#nm.1.1.1.1.2, (#nm.1.1.1.2, (nm.1.1.2, (#nm.1.2, (#nm.2, #())))))))))))))))))))%V) by f_equal.
       unfold tuple_of. simpl TypeVector.tuple_of. iApply "HΦ". subst b ns nm.
-      iExists 0%nat. iExists 0%nat.
       unfold coq_processClientRequest. rewrite Heqb. simpl. iFrame.
       unfold is_message; simplNotation; simpl. iClear "H_reply". repeat (iSplit; try done).
       iSplitL "". { iApply own_slice_small_nil. done. } repeat (iSplit; try done).
@@ -53,7 +49,7 @@ Section heap.
         wp_apply (wp_storeField_struct with "[H_reply]"). { repeat econstructor; eauto. } { iExact "H_reply". } iIntros "H_reply". wp_pures.
         wp_apply (wp_getDataFromOperationLog with "[$H6]"). iIntros "%r (-> & H6)".
         wp_apply (wp_storeField_struct with "[H_reply]"). { repeat econstructor; eauto. } { iExact "H_reply". } iIntros "H_reply". wp_pures.
-        wp_apply (wp_NewSlice). iIntros "%s1 H_s1". replace (replicate (uint.nat (W64 0)) u64_IntoVal .(IntoVal_def w64)) with ( @nil u64) by reflexivity.
+        wp_apply (wp_NewSlice). iIntros "%s1 H_s1". replace (replicate (uint.nat (W64 0)) u64_IntoVal .(IntoVal_def w64)) with ( @nil u64 ) by reflexivity.
         wp_apply (wp_SliceAppendSlice with "[$H_s1 $H4]"); auto. clear s1. iIntros "%s1 [H_s1 H4]". simpl.
         wp_apply (wp_storeField_struct with "[H_reply]"). { repeat econstructor; eauto. } { iExact "H_reply". } iIntros "H_reply". wp_pures.
         wp_apply (wp_storeField_struct with "[H_reply]"). { repeat econstructor; eauto. } { iExact "H_reply". } iIntros "H_reply". wp_pures.
@@ -64,7 +60,6 @@ Section heap.
         set (nm := (W64 4, W64 0, W64 0, W64 0, W64 0, Slice.nil, W64 0, W64 0, Slice.nil, W64 0, W64 0, W64 0, W64 0, W64 0, coq_getDataFromOperationLog s .(Server.OperationsPerformed), s1, s .(Server.Id), msg .(Message.C2S_Client_Id))).
         replace (Φ (#true, (#s .(Server.Id), (#s .(Server.NumberOfServers), (t4, (t3, (t2, (t1, (t0, (t, #())))))))), (#(W64 4), (zero_val uint64T, (zero_val uint64T, (zero_val uint64T, (zero_val uint64T, (zero_val (slice.T uint64T), (zero_val uint64T, (zero_val uint64T, (zero_val (slice.T (slice.T uint64T * (uint64T * unitT)%ht)), (zero_val uint64T, (zero_val uint64T, (zero_val uint64T, (zero_val uint64T, (#(W64 0), (#(coq_getDataFromOperationLog s .(Server.OperationsPerformed)), (s1, (#s .(Server.Id), (#msg .(Message.C2S_Client_Id), #())))))))))))))))))))%V) with (Φ (#b, server_val ns, message_val nm)%V) by f_equal.
         unfold server_val, message_val. iApply "HΦ". subst b ns nm.
-        iExists 0%nat. iExists (length s .(Server.VectorClock)).
         unfold coq_processClientRequest; rewrite Heqb; simpl.
         assert ((uint.nat msg .(Message.C2S_Client_OperationType) =? 0) = true) as H_OBS1.
         { rewrite Z.eqb_eq. word. }
@@ -91,18 +86,23 @@ Section heap.
         wp_load. wp_pures. wp_apply (wp_SliceGet with "[$H4]"); auto. iIntros "H4".
         wp_load. wp_pures. wp_apply (wp_SliceSet with "[$H4]"); auto. iIntros "H4".
         wp_pures. wp_apply (wp_NewSlice). iIntros "%s2 H_s2". wp_apply (wp_SliceAppendSlice with "[$H_s2 $H4]"); auto.
-        clear s2. iIntros "%s2 [H_s2 H4]". replace (replicate (uint.nat (W64 0)) u64_IntoVal .(IntoVal_def w64)) with ( @nil w64) by reflexivity. simpl.
+        clear s2. iIntros "%s2 [H_s2 H4]". replace (replicate (uint.nat (W64 0)) u64_IntoVal .(IntoVal_def w64)) with ( @nil w64 ) by reflexivity. simpl.
+        iDestruct "H_s2" as "[H1_s2 H2_s2]". iMod (own_slice_small_persist with "[$H1_s2]") as "H1_s2".
         wp_pures. wp_load. wp_pures. replace (s2, (#msg .(Message.C2S_Client_Data), #()))%V with (to_val (s2, msg .(Message.C2S_Client_Data))) by reflexivity.
-        iDestruct "H6" as "(%t2_ops & H6 & H_t2_ops)". wp_apply (wp_SliceAppend with "[$H6]"). iIntros "%s3 H_s3".
+        iDestruct "H6" as "(%t2_ops & H6 & H_t2_ops)". wp_apply (another_wp_sortedInsert with "[$H6 $H_t2_ops H1_s2]"). { instantiate (1 := {| Operation.VersionVector := (<[uint.nat s .(Server.Id):=w64_word_instance .(word.add) x (W64 1)]> s .(Server.VectorClock)); Operation.Data := msg .(Message.C2S_Client_Data); |}). apply list_lookup_total_correct in H_x. subst x. unfold lookup_total. iFrame. rewrite length_insert. done. } iIntros "%s3 (H_s3 & %H1_sorted)".
         wp_pures. wp_apply (wp_storeField_struct with "[H_s1]"). { repeat econstructor; eauto. } { iExact "H_s1". } iIntros "H_s1".
         wp_pures. wp_load. wp_pures. replace (SliceAppendSlice uint64T slice.nil t3) with (SliceAppendSlice uint64T Slice.nil t3) by reflexivity.
-        wp_apply (wp_SliceAppendSlice with "[H4]"). { repeat econstructor; eauto. }
-        { iSplitL "".
-          - unfold own_slice. instantiate (1 := @nil u64). simpl list.untype. iApply own_slice_nil; done.
-          - iExact "H4".
+        wp_apply (wp_SliceAppendSlice with "[H4]"). { repeat econstructor; eauto. } { instantiate (5 := @nil u64). iSplitR "H4"; try done. iApply own_slice_nil; done. } iIntros "%s4 [H_s4 H4]".
+        iDestruct "H7" as "(%t1_ops & H7 & H_t1_ops)". iDestruct "H_s4" as "[H1_s4 H2_s4]". iMod (own_slice_small_persist with "[$H1_s4]") as "H1_s4".
+        wp_load. wp_pures. replace (s4, (#msg .(Message.C2S_Client_Data), #()))%V with (to_val (s4, msg .(Message.C2S_Client_Data))) by reflexivity. simpl.
+        wp_apply (another_wp_sortedInsert with "[H7 H_t1_ops H1_s4]").
+        { iSplitL "H7 H_t1_ops".
+          - iExists t1_ops. iFrame.
+          - instantiate (1 := {| Operation.VersionVector := (<[uint.nat s .(Server.Id):=w64_word_instance .(word.add) x (W64 1)]> s .(Server.VectorClock)); Operation.Data := msg .(Message.C2S_Client_Data); |}). simpl. iSplitL "H1_s4".
+            + iFrame. rewrite length_insert. done.
+            + done.
         }
-        simpl. iIntros "%s4 [H_s4 H4]". wp_load. wp_pures. replace (s4, (#msg .(Message.C2S_Client_Data), #()))%V with (to_val (s4, msg .(Message.C2S_Client_Data))) by reflexivity.
-        iDestruct "H7" as "(%t1_ops & H7 & H_t1_ops)". wp_apply (wp_SliceAppend with "[$H7]"). iIntros "%s5 H_s5". wp_apply (wp_storeField_struct with "[H_s1]"). { repeat econstructor; eauto. } { iExact "H_s1". } iIntros "H_s1".
+        iIntros "%s5 (H_s5 & %H2_sorted)". wp_apply (wp_storeField_struct with "[H_s1]"). { repeat econstructor; eauto. } { iExact "H_s1". } iIntros "H_s1".
         wp_pures. wp_apply (wp_storeField_struct with "[H_reply]"); eauto. simpl. iIntros "H_reply".
         wp_pures. wp_apply (wp_storeField_struct with "[H_reply]"); eauto. simpl. iIntros "H_reply".
         wp_pures. wp_apply (wp_storeField_struct with "[H_reply]"); eauto. simpl. iIntros "H_reply".
@@ -112,21 +112,18 @@ Section heap.
         wp_pures. wp_apply (wp_storeField_struct with "[H_reply]"); eauto. simpl. iIntros "H_reply".
         wp_pures. wp_apply (wp_storeField_struct with "[H_reply]"); eauto. simpl. iIntros "H_reply".
         wp_pures. wp_load. wp_pures. wp_load. wp_pures.
-        iDestruct "H_s2" as "[H1_s2 H2_s2]". iMod (own_slice_small_persist with "[$H1_s2]") as "H1_s2".
-        iDestruct "H_s4" as "[H1_s4 H2_s4]". iMod (own_slice_small_persist with "[$H1_s4]") as "H1_s4".
         iModIntro.
         pose (b := true).
         set (ns := (s .(Server.Id), s .(Server.NumberOfServers), t4, t3, s3, s5, t0, t)).
         set (nm := (W64 4, W64 0, W64 0, W64 0, W64 0, Slice.nil, W64 0, W64 0, Slice.nil, W64 0, W64 0, W64 0, W64 0, W64 1, W64 0, s6, s .(Server.Id), msg .(Message.C2S_Client_Id))).
         replace (Φ (#true, (#s .(Server.Id), (#s .(Server.NumberOfServers), (t4, (t3, (s3, (s5, (t0, (t, #())))))))), (#(W64 4), (zero_val uint64T, (zero_val uint64T, (zero_val uint64T, (zero_val uint64T, (zero_val (slice.T uint64T), (zero_val uint64T, (zero_val uint64T, (zero_val (slice.T (slice.T uint64T * (uint64T * unitT)%ht)), (zero_val uint64T, (zero_val uint64T, (zero_val uint64T, (zero_val uint64T, (#(W64 1), (#(W64 0), (s6, (#s .(Server.Id), (#msg .(Message.C2S_Client_Id), #())))))))))))))))))))%V) with (Φ (#b, server_val ns, message_val nm)%V) by f_equal.
         unfold server_val, message_val. iApply "HΦ". subst b ns nm. simpl.
-        iExists 0%nat. iExists (length s .(Server.VectorClock)).
         unfold coq_processClientRequest; rewrite Heqb; simpl.
         assert ((uint.nat msg .(Message.C2S_Client_OperationType) =? 0) = false) as H_OBS1.
         { rewrite Z.eqb_neq. word. }
         rewrite H_OBS1; simpl. unfold is_message; simplNotation; simpl. rewrite Z.eqb_neq in H_OBS1.
         iSplitL "". { done. }
-        iSplitL "H3 H4 H1_s2 H_s3 H1_s4 H_s5 H8 H9 H_t2_ops H_t1_ops".
+        iSplitL "H3 H4 H_s3 H_s5 H8 H9".
         { apply list_lookup_total_correct in H_x. subst x. unfold lookup_total.
           replace (w64_word_instance .(word.add) (list_lookup_total (uint.nat s .(Server.Id)) s .(Server.VectorClock)) (W64 1)) with (W64 (uint.nat (list_lookup_total (uint.nat s .(Server.Id)) s .(Server.VectorClock)) + 1)) in * by word.
           iFrame; simpl; simplNotation. repeat rewrite length_insert. repeat (iSplit; try done).
@@ -134,7 +131,7 @@ Section heap.
         repeat rewrite length_insert.
         iSplitL "H_s6".
         { apply list_lookup_total_correct in H_x. subst x. unfold lookup_total.
-          replace (replicate (uint.nat (W64 0)) (W64 0)) with ( @nil u64) by reflexivity. simpl.
+          replace (replicate (uint.nat (W64 0)) (W64 0)) with ( @nil u64 ) by reflexivity. simpl.
           replace (w64_word_instance .(word.add) (list_lookup_total (uint.nat s .(Server.Id)) s .(Server.VectorClock)) (W64 1)) with (W64 (uint.nat (list_lookup_total (uint.nat s .(Server.Id)) s .(Server.VectorClock)) + 1)) by word.
           repeat (iSplit; try done). iSplitL "". { iApply own_slice_small_nil; eauto. }
           repeat (iSplit; try done). iSplitL "".
@@ -146,88 +143,31 @@ Section heap.
         }
         iSplitL "H20 H27 H16".
         { iFrame. done. }
-        iSplit; try done.
-        iPureIntro. intros (H1_SORTED & H2_SORTED). split.
-        { simpl; trivial. }
-        { simpl. intros i j i_lt_j x1 x2 H_x1 H_x2.
-          assert (j < length ((s .(Server.OperationsPerformed) ++ [ {| Operation.VersionVector := <[uint.nat s .(Server.Id):=W64 (uint.nat (list_lookup_total (uint.nat s .(Server.Id)) s .(Server.VectorClock)) + 1)]> s .(Server.VectorClock); Operation.Data := msg .(Message.C2S_Client_Data) |}])))%nat as j_bound.
-          { eapply lookup_lt_is_Some_1. exists x2; trivial. }
-          rewrite length_app in j_bound. simpl in *.
-          assert (j = length s.(Server.OperationsPerformed) \/ j < length s.(Server.OperationsPerformed))%nat as [EQ | LT] by word.
-          - subst j. rewrite lookup_snoc in H_x2.
-            assert (x2 = {| Operation.VersionVector := <[uint.nat s .(Server.Id):=W64 (uint.nat (list_lookup_total (uint.nat s .(Server.Id)) s .(Server.VectorClock)) + 1)]> s .(Server.VectorClock); Operation.Data := msg .(Message.C2S_Client_Data) |}) as -> by congruence.
-            clear H_x2 j_bound; simpl. apply list_lookup_total_correct in H_x. subst x. rewrite lookup_app_l in H_x1; cycle 1. { word. }
-            set (lhs := (<[uint.nat s .(Server.Id):=W64 (uint.nat (list_lookup_total (uint.nat s .(Server.Id)) s .(Server.VectorClock)) + 1)]> s .(Server.VectorClock))).
-            set (rhs := x1 .(Operation.VersionVector)).
-            
-        }
-  Qed. *) Admitted.
+        apply list_lookup_total_correct in H_x. subst x. unfold lookup_total in *.
+        replace (w64_word_instance .(word.add) (list_lookup_total (uint.nat s .(Server.Id)) s .(Server.VectorClock)) (W64 1)) with (W64 (uint.nat (list_lookup_total (uint.nat s .(Server.Id)) s .(Server.VectorClock)) + 1)) in * by word.
+        iPureIntro. split; simpl; trivial.
+        rewrite length_insert. word.
+  Qed.
 
-  Definition coq_processRequest (server : Server.t) (request : Message.t) : Server.t * list Message.t :=
-    match uint.nat request.(Message.MessageType) with
-    | 0%nat =>
-        let '(succeeded, server, reply) := coq_processClientRequest server request in
-        if succeeded then
-          (server, [reply])
-        else
-          let UnsatisfiedRequests := server.(Server.UnsatisfiedRequests) ++ [request] in 
-          let server := Server.mk server.(Server.Id) server.(Server.NumberOfServers) UnsatisfiedRequests server.(Server.VectorClock) server.(Server.OperationsPerformed) server.(Server.MyOperations) server.(Server.PendingOperations) server.(Server.GossipAcknowledgements) in
-          (server, [])
-    | 1%nat =>
-        let server := coq_receiveGossip server request in
-        let focus := server.(Server.UnsatisfiedRequests) in
-        let loop_init : nat * (Server.t * list Message.t) :=
-          (0%nat, (server, [Message.mk 0 0 0 0 0 [] 0 0 [] 0 (server.(Server.Id)) (request.(Message.S2S_Gossip_Sending_ServerId)) (request.(Message.S2S_Gossip_Index)) 0 0 [] 0 0]))
-        in
-        let loop_step (acc: nat * (Server.t * list Message.t)) (element: Message.t) : nat * (Server.t * list Message.t) :=
-          let '(i, (s, outGoingRequests)) := acc in
-          let '(succeeded, s, reply) := coq_processClientRequest s element in
-          if succeeded then
-            let UnsatisfiedRequests := coq_deleteAtIndexMessage s.(Server.UnsatisfiedRequests) i in
-            (i, (Server.mk s.(Server.Id) s.(Server.NumberOfServers) UnsatisfiedRequests s.(Server.VectorClock) s.(Server.OperationsPerformed) s.(Server.MyOperations) s.(Server.PendingOperations) s.(Server.GossipAcknowledgements), outGoingRequests ++ [reply]))
-          else
-            ((i + 1)%nat, (s, outGoingRequests))
-        in
-        snd (fold_left loop_step focus loop_init)
-    | 2%nat => (coq_acknowledgeGossip server request, [])
-    | 3%nat =>
-      let loop_init : list Message.t :=
-        []
-      in
-      let loop_step (acc: list Message.t) (index: nat) : list Message.t :=
-        if (negb (index =? (uint.nat server.(Server.Id)))) then
-          let S2S_Gossip_Sending_ServerId := server.(Server.Id) in
-          let S2S_Gossip_Receiving_ServerId := index in
-          let S2S_Gossip_Operations := coq_getGossipOperations server index in
-          let S2S_Gossip_Index := length (server.(Server.MyOperations)) in
-          let message := Message.mk 1 0 0 0 0 [] S2S_Gossip_Sending_ServerId S2S_Gossip_Receiving_ServerId S2S_Gossip_Operations S2S_Gossip_Index 0 0 0 0 0 [] 0 0 in
-          acc ++ [message]
-        else
-          acc
-      in
-      (server, fold_left loop_step (seq 0%nat (uint.nat server.(Server.NumberOfServers))) loop_init)
-    | _ => (server, [])
-    end.
-
-  Lemma wp_processRequest sv s msgv msg (n: nat) (m: nat) len_po len_ga len_s2c :
+  Lemma wp_processRequest sv s msgv msg (n: nat) (m: nat) len_po len_ga len_c2s len_s2c :
     {{{
         is_server sv s n m m m len_po len_ga ∗
-        is_message msgv msg n m len_s2c ∗
-        ⌜SERVER_INVARIANT s⌝
+        is_message msgv msg n len_c2s len_s2c ∗
+        ⌜m = len_c2s /\ INVARIANT.SERVER s⌝
     }}}
       processRequest (server_val sv) (message_val msgv)
     {{{
         ns nms, RET (server_val ns, slice_val nms);
         is_server ns (coq_processRequest s msg).1 n m m m len_po len_ga ∗
         message_slice nms (coq_processRequest s msg).2 n ∗
-        ⌜SERVER_INVARIANT (coq_processRequest s msg).1⌝
+        ⌜INVARIANT.SERVER (coq_processRequest s msg).1⌝
     }}}.
   Proof. (**
     assert (rewrite_nil : forall A : Type, forall x : A, forall n : nat, n = 0%nat -> replicate n x = []) by now intros; subst; reflexivity.
     rewrite redefine_server_val redefine_message_val. TypeVector.des sv. TypeVector.des msgv. iIntros "%Φ (H_server & H_message & %H_precondition) HΦ".
     iDestruct "H_server" as "(%H1 & %H2 & H3 & H4 & %H5 & H6 & H7 & H8 & H9 & %H10)".
     iDestruct "H_message" as "(%H11 & %H12 & %H13 & %H14 & %H15 & H16 & %H17 & %H18 & %H19 & H20 & %H21 & %H22 & %H23 & %H24 & %H25 & %H26 & H27 & %H28 & %H29 & %H30)".
-    unfold SERVER_INVARIANT in *. destruct H_precondition as (H1_precondition & H2_precondition & H3_precondition); simplNotation; subst; rewrite /processRequest.
+    unfold INVARIANT.SERVER in *. destruct H_precondition as (H1_precondition & H2_precondition & H3_precondition); simplNotation; subst; rewrite /processRequest.
     wp_pures. wp_apply wp_NewSlice. simpl. rewrite rewrite_nil; cycle 1. { word. } iIntros "%s1 H_s1".
     wp_pures. wp_apply wp_ref_to. { repeat econstructor; eauto. } iIntros "%outGoingRequests H_outGoingRequests".
     wp_pures. wp_apply wp_ref_to. { repeat econstructor; eauto. } iIntros "%server H_server".
@@ -241,7 +181,7 @@ Section heap.
       - wp_load. wp_load. replace message_val with (message_into_val .(to_val)) by reflexivity. wp_apply (wp_SliceAppend with "[$H_s1]"). iIntros "%s2 H_s2".
         wp_store. wp_load. wp_load. wp_pures. simpl. iModIntro. iApply "HΦ".
         unfold coq_processRequest; rewrite Heqb; replace (uint.nat (W64 0)) with 0%nat by reflexivity. destruct (coq_processClientRequest s msg) as [[succeeded_v s_v] reply_v] eqn: H_OBS; simpl in *.
-        destruct H1_postcondition as [-> ->]; subst succeeded_v; simpl in *. iFrame. simp.
+        destruct H1_postcondition as [-> ->]; subst succeeded_v; simpl in *. iFrame. simpl.
       - wp_load. wp_pures. iDestruct "H_server'" as "(%H1 & %H2 & H3 & H4 & %H5 & H6 & H7 & H8 & H9 & %H10)". iDestruct "H_message'" as "(%H11 & %H12 & %H13 & %H14 & %H15 & H16 & %H17 & %H18 & %H19 & H20 & %H21 & %H22 & %H23 & %H24 & %H25 & %H26 & H27 & %H28 & %H29 & %H30)". simplNotation; subst.
         replace (#msg .(Message.MessageType), (#msg .(Message.C2S_Client_Id), (#msg .(Message.C2S_Server_Id), (#msg .(Message.C2S_Client_OperationType), (#msg .(Message.C2S_Client_Data), (t7, (#msg .(Message.S2S_Gossip_Sending_ServerId), (#msg .(Message.S2S_Gossip_Receiving_ServerId), (t6, (#msg .(Message.S2S_Gossip_Index), (#msg .(Message.S2S_Acknowledge_Gossip_Sending_ServerId), (#msg .(Message.S2S_Acknowledge_Gossip_Receiving_ServerId), (#msg .(Message.S2S_Acknowledge_Gossip_Index), (#msg .(Message.S2C_Client_OperationType), (#msg .(Message.S2C_Client_Data), (t5, (#msg .(Message.S2C_Server_Id), (#msg .(Message.S2C_Client_Number), #()))))))))))))))))))%V with (message_into_val .(to_val) (msg .(Message.MessageType), msg .(Message.C2S_Client_Id), msg .(Message.C2S_Server_Id), msg .(Message.C2S_Client_OperationType), msg .(Message.C2S_Client_Data), t7, msg .(Message.S2S_Gossip_Sending_ServerId), msg .(Message.S2S_Gossip_Receiving_ServerId), t6, msg .(Message.S2S_Gossip_Index), msg .(Message.S2S_Acknowledge_Gossip_Sending_ServerId), msg .(Message.S2S_Acknowledge_Gossip_Receiving_ServerId), msg .(Message.S2S_Acknowledge_Gossip_Index), msg .(Message.S2C_Client_OperationType), msg .(Message.S2C_Client_Data), t5, msg .(Message.S2C_Server_Id), msg .(Message.S2C_Client_Number))) by reflexivity.
         iDestruct "H3" as "(%ops1 & H3 & H_ops1)". wp_apply (wp_SliceAppend with "[$H3]"). iIntros "%s2 H_s2". wp_apply (wp_storeField_struct with "[H_server]"); auto. iIntros "H_server".
